theories/laws/utp_rename_laws.thy
@@ -15,6 +15,110 @@ imports
   "../tactics/utp_expr_tac"
 begin
 
+subsubsection {* Predicate Laws *}
+
+theorem EvalP_RenameP [eval] :
+"\<lbrakk>p[ss]\<rbrakk>b = \<lbrakk>p\<rbrakk>(RenameB (inv\<^sub>s ss) b)"
+apply (simp add: EvalP_def)
+apply (simp add: RenameP_def)
+apply (simp add: image_def)
+apply (safe)
+apply (simp)
+apply (rule_tac x = "RenameB (inv\<^sub>s ss) b" in bexI)
+apply (simp)
+apply (assumption)
+done
+
+theorem EvalP_RenamePMap_one [eval] :
+"\<lbrakk> x \<noteq> x'; vtype x' = vtype x; aux x' = aux x \<rbrakk> \<Longrightarrow>
+ \<lbrakk>p\<^bsup>[x \<mapsto> x']\<^esup>\<rbrakk>b = \<lbrakk>p\<rbrakk>(b(x :=\<^sub>b \<langle>b\<rangle>\<^sub>b x', x' :=\<^sub>b \<langle>b\<rangle>\<^sub>b x))"
+apply (simp add: RenamePMap_def)
+apply (simp add: eval closure)
+apply (simp add: EvalP_def)
+apply (simp add: RenameP_def RenameB_def image_def closure)
+apply (simp add: MapR_rep_eq[of "[x]" "[x']",simplified] CompB_def)
+apply (subgoal_tac "Abs_WF_BINDING (\<langle>b\<rangle>\<^sub>b \<circ> MapRename [x \<mapsto> x']) = b(x :=\<^sub>b \<langle>b\<rangle>\<^sub>b x', x' :=\<^sub>b \<langle>b\<rangle>\<^sub>b x)")
+apply (simp add: closure)
+apply (rule Rep_WF_BINDING_intro)
+apply (simp add:closure)
+apply (subgoal_tac "\<langle>b\<rangle>\<^sub>b x \<rhd> x'")
+apply (simp)
+apply (rule ext)
+apply (simp add: MapRename_def closure)
+apply (auto)
+done
+
+theorem RenameP_id :
+"p[id\<^sub>s] = p"
+apply (utp_pred_auto_tac)
+done
+
+theorem RenameP_inverse1 :
+"p[ss][inv\<^sub>s ss] = p"
+apply (utp_pred_auto_tac)
+done
+
+theorem RenameP_inverse2 :
+"p[inv\<^sub>s ss][ss] = p"
+apply (utp_pred_auto_tac)
+done
+
+theorem RenameP_compose :
+"p[ss1][ss2] = RenameP p (ss2 \<circ>\<^sub>s ss1)"
+apply (utp_pred_tac)
+apply (simp add: RenameB_compose closure)
+done
+
+theorem RenameP_commute :
+"\<lbrakk>ss1 \<in> VAR_RENAME_ON vs1;
+ ss2 \<in> VAR_RENAME_ON vs2;
+ vs1 \<inter> vs2 = {}\<rbrakk> \<Longrightarrow>
+ (p::'VALUE WF_PREDICATE)[ss1][ss2] = p[ss2][ss1]"
+apply (utp_pred_tac)
+apply (clarify)
+apply (subst RenameB_commute [of "(inv\<^sub>s ss1)" "vs1" "(inv\<^sub>s ss2)" "vs2" "b"])
+apply (simp_all add: closure)
+done
+
+theorem RenameP_involution [simp] :
+"\<lbrakk>ss \<in> VAR_RENAME_INV\<rbrakk> \<Longrightarrow>
+ p[ss][ss] = p"
+apply (utp_pred_auto_tac)
+done
+
+theorems rename_simps =
+  RenameP_id
+  RenameP_inverse1
+  RenameP_inverse2
+  RenameP_compose
+  RenameP_involution
+
+declare rename_simps [urename]
+
+subsection {* Distribution theorems *}
+
+theorem RenameP_image_union [urename]:
+  "\<langle>ss\<rangle>\<^sub>s ` (vs1 \<union> vs2) = \<langle>ss\<rangle>\<^sub>s ` vs1 \<union> \<langle>ss\<rangle>\<^sub>s ` vs2"
+  by auto
+
+theorem RenameP_image_inter [urename]:
+  "\<langle>ss\<rangle>\<^sub>s ` (vs1 \<inter> vs2) = \<langle>ss\<rangle>\<^sub>s ` vs1 \<inter> \<langle>ss\<rangle>\<^sub>s ` vs2"
+  by (auto, metis Rep_VAR_RENAME VAR_RENAME_in_image)
+
+theorem RenameP_image_minus [urename]:
+  "\<langle>ss\<rangle>\<^sub>s ` (vs1 - vs2) = \<langle>ss\<rangle>\<^sub>s ` vs1 - \<langle>ss\<rangle>\<^sub>s ` vs2"
+  by (metis Rep_VAR_RENAME_inj image_set_diff)
+ 
+lemma RenameP_image_uminus [urename]: 
+  "\<langle>ss\<rangle>\<^sub>s ` (- vs) = - (\<langle>ss\<rangle>\<^sub>s ` vs)"
+  by (metis (lifting) Rep_VAR_RENAME_bij bij_image_Compl_eq) 
+
+theorems rename_dist =
+  RenameP_image_union
+  RenameP_image_inter
+  RenameP_image_minus
+  RenameP_image_uminus
+
 subsubsection {* Predicate Renaming Theorems *}
 
 theorem RenameP_NotP_distr [urename]:
