theories/poly/utp_poly_value.thy
@@ -1,0 +1,168 @@
+(******************************************************************************)
+(* Project: Unifying Theories of Programming in HOL                           *)
+(* File: utp_poly_value.thy                                                   *)
+(* Author: Simon Foster, University of York (UK)                              *)
+(******************************************************************************)
+
+header {* Shallow Polymorphic Values *}
+
+theory utp_poly_value
+imports 
+  "../core/utp_value"
+  "../core/utp_sorts"
+  "../core/utp_event"
+begin
+
+default_sort type
+
+subsection {* Polymorphic constants *}
+
+text {* The following global constants serve to link the (polymorphic)
+        HOL types which we would like to use in UTP predicates /
+        expressions with the (also polymorphic) model type. Since we
+        need range over these two type variables we cannot use a
+        type-class, which are limited to one variable for reasons of
+        guaranteeing decidability. Isabelle constants provide a way to
+        directly create polymorphic functions, but a great deal of
+        care is needed in using them. If associated definitions for
+        the constants overlap chaos will ensue, as the type-system may
+        not be able to disambiguate. FIXME: We need to defined some
+        carefully thought rules to define what we can and can't have here. 
+*}
+
+consts 
+  TypeU :: "'a itself \<Rightarrow> ('m :: VALUE) UTYPE"
+  InjU  :: "'a \<Rightarrow> 'm :: VALUE"
+  ProjU :: "'m :: VALUE \<Rightarrow> 'a"
+
+text {* @{const TypeU} gives the corresponding UTP model type for a
+        given HOL type, effectively performing an erasure. @{const
+        InjU} injects a HOL value into a given model, and @{const
+        ProjU} is the inverse. *}
+
+text {* At this point we could add axioms about our consts, but since
+        these are user checked I consider this too dangerous to the integrity of 
+        the Isabelle/UTP model. Instead we create the following definition
+        which encodes the required constraints over the constants, and will need
+        to be added as assumptions to proofs about definitions which use these 
+        constants. Without this we know nothing about the behaviour of constants. *}
+
+definition TypeUSound :: "'a itself \<Rightarrow> 'm::VALUE itself \<Rightarrow> bool" where
+"TypeUSound a m \<longleftrightarrow> (\<forall> (x :: 'a). (InjU x :: 'm) :! TypeU a) \<and>
+                    (\<forall> (x :: 'a). (ProjU (InjU x :: 'm) = x))"
+
+syntax
+  "_TYPEU"      :: "type => logic"  ("(1TYPEU/(1'(_')))")
+  "_TYPEUSOUND" :: "type \<Rightarrow> type => logic"  ("(1TYPEUSOUND/(1'(_, _')))")
+
+translations 
+  "TYPEUSOUND('a, 'm)" == "CONST TypeUSound TYPE('a) TYPE('m)"
+  "TYPEU('a)" == "CONST TypeU TYPE('a)"
+
+text {* @{const TypeUSound} can be thought of as a two-parameter type
+        class which stores the properties of the above polymorphic
+        constants, namely that the given Isabelle type can be
+        constructed under the given sort constraints. For instance we could
+        declare @{term "TYPEUSOUND(int, 'm :: INT_SORT)"}. *}
+
+text {* The following defs are carefully crafted, there must no
+        overlap or \emph{potential} overlap.  That is to say it must
+        not be possible to create a type class or instance which
+        renders them undisambiguable.  Basically the LHS (value type)
+        of @{const InjU} / @{const TypeU} should define the
+        \emph{concrete type} which is to mapped. It can be parametric,
+        but I can't conceive of a situation when this would be a class
+        constraint -- I believe this would wreck the type system. This
+        given, the RHS (model type) can then consist of only sort
+        constraints. For instance for @{typ bool} the value type is of
+        course @{typ bool} and the model type is @{typ "'m ::
+        BOOL_SORT"}, since we need the ability to reconstruct the
+        boolean in the model. Nevertheless these definitions
+        \emph{are} extensible, but a great deal of care is required! *}
+
+defs (overloaded)
+  InjU_bool [simp]:  "InjU (x::bool) \<equiv> MkBool x"
+  ProjU_bool [simp]: "ProjU (x::('a::BOOL_SORT)) \<equiv> DestBool x"
+  TypeU_bool [simp]: "TypeU (x::bool itself) \<equiv> BoolType"
+
+  InjU_int [simp]:  "InjU (x::int) \<equiv> MkInt x"
+  ProjU_int [simp]: "ProjU (x::('a::INT_SORT)) \<equiv> DestInt x"
+  TypeU_int [simp]: "TypeU (x::int itself) \<equiv> IntType"
+
+  InjU_event [simp]:  "InjU (x::('m::EVENT_SORT) EVENT) \<equiv> (MkEvent x::'m)"
+  ProjU_event [simp]: "ProjU (x::('m::EVENT_SORT)) \<equiv> DestEvent x"
+  TypeU_event [simp]: "TypeU (x::('m::EVENT_SORT) EVENT itself) \<equiv> EventType::'m UTYPE"
+
+  InjU_list [simp]: "InjU (xs::'a list) \<equiv> MkList (TypeU (TYPE('a))) (map InjU xs)"
+  ProjU_list [simp]: "ProjU (xs::('a::LIST_SORT)) \<equiv> map ProjU (DestList xs)"
+  TypeU_list [simp]: "TypeU (x::('a list) itself) \<equiv> ListType (TypeU TYPE('a))"
+
+  InjU_fset [simp]: "InjU (xs::'a fset) \<equiv> MkFSet (TypeU (TYPE('a))) (InjU `\<^sub>f xs)"
+  ProjU_fset [simp]: "ProjU (xs::('a::FSET_SORT)) \<equiv> ProjU `\<^sub>f (DestFSet xs)"
+  TypeU_fset [simp]: "TypeU (x::('a fset) itself) \<equiv> FSetType (TypeU TYPE('a))"  
+
+subsection {* @{const TypeUSound} rules *}
+
+lemma TypeUSound_intro [intro]:
+  "\<lbrakk> \<And> (x :: 'a). (InjU x :: 'm) :! TYPEU('a)
+   ; \<And> (x :: 'a). (ProjU (InjU x :: 'm) = x) \<rbrakk> \<Longrightarrow>
+   TYPEUSOUND('a, 'm :: VALUE)"
+  by (simp add:TypeUSound_def)
+
+lemma TypeUSound_InjU_type [typing]:
+  fixes x :: "'a"
+  assumes "TYPEUSOUND('a, 'm :: VALUE)"
+  shows "(InjU x :: 'm) :! TYPEU('a)"
+  using assms by (auto simp add:TypeUSound_def)
+
+lemma TypeUSound_InjU_defined [defined]:
+  fixes x :: "'a"
+  assumes "TYPEUSOUND('a, 'm :: VALUE)"
+  shows "\<D> (InjU x :: 'm)"
+  by (auto intro:assms typing defined)
+
+lemma TypeUSound_InjU_inv [simp]:
+  fixes x :: "'a"
+  assumes "TYPEUSOUND('a, 'm :: VALUE)"
+  shows "ProjU (InjU x :: 'm) = x"
+  using assms by (auto simp add:TypeUSound_def)
+
+subsection {* Some basic instantiations *}
+
+text {* The following instantiations make use of the sort constraints
+        to discharge the requirements of @{const TypeUSound}. *}
+
+lemma TypeUSound_bool [typing]: "TYPEUSOUND(bool, 'm :: BOOL_SORT)"
+  by (simp add:TypeUSound_def typing)
+
+lemma TypeUSound_int [typing]: "TYPEUSOUND(int, 'm :: INT_SORT)"
+  by (simp add:TypeUSound_def typing)
+
+lemma TypeUSound_list [typing]: 
+  "\<lbrakk> (TYPEU('a) :: 'm UTYPE) \<in> ListPerm; TYPEUSOUND('a, 'm) \<rbrakk> 
+     \<Longrightarrow> TYPEUSOUND('a list, 'm :: LIST_SORT)"
+  apply (auto simp add:dcarrier_def TypeUSound_def)
+  apply (rule typing, auto)
+  apply (subgoal_tac "set (map InjU x) \<subseteq> dcarrier (TYPEU('a) :: 'm UTYPE)")
+  apply (auto simp add:comp_def)
+done
+
+lemma TypeUSound_fset [typing]: 
+  "\<lbrakk> (TYPEU('a) :: 'm UTYPE) \<in> FSetPerm; TYPEUSOUND('a, 'm) \<rbrakk> 
+     \<Longrightarrow> TYPEUSOUND('a fset, 'm :: FSET_SORT)"
+  apply (simp add:dcarrier_def TypeUSound_def)
+  apply (rule)
+  apply (clarify)
+  apply (rule typing)
+  apply (force)
+  apply (force)
+  apply (clarify)
+  apply (subgoal_tac "\<langle>InjU `\<^sub>f x\<rangle>\<^sub>f \<subseteq> dcarrier (TYPEU('a) :: 'm UTYPE)")
+  apply (auto simp add:image_def)
+done
+
+lemma TypeUSound_Event [typing]:
+  "TYPEUSOUND('m EVENT, 'm :: EVENT_SORT)"
+  by (auto simp add:typing)
+
+end
