theories/poly/utp_poly_var.thy
@@ -1,0 +1,110 @@
+(******************************************************************************)
+(* Project: Unifying Theories of Programming in HOL                           *)
+(* File: utp_poly_var.thy                                                     *)
+(* Author: Simon Foster, University of York (UK)                              *)
+(******************************************************************************)
+
+header {* Shallowly Embedded Polymorphic Variables *}
+
+theory utp_poly_var
+imports 
+  "../core/utp_var"
+  "../core/utp_rename"
+  utp_poly_value
+begin
+
+default_sort type
+
+subsection {* Polymorphic type variables *}
+
+text {* A derivative of normal variables @{typ "'m VAR"} which also carry 
+        their HOL type. They are not and cannot be a replacement
+        because the HOL type-system does not allow sets of heterogeneous
+        values, hence alphabets remain sets of deep variables. But whenever
+        they can be used the advantage is that the HOL type-system can
+        help the proof processes by discharging the type constraints.
+
+        At first glance this type may seem odd as it refers to two
+        type variables which are not used internally. This is because
+        these are simply there to help the type-system and store no
+        additional data. *}
+
+typedef ('a, 'm :: VALUE) PVAR = "UNIV :: (NAME * bool) set"
+  by auto
+
+declare Rep_PVAR [simp]
+declare Rep_PVAR_inverse [simp]
+declare Abs_PVAR_inverse [simp]
+
+definition MkPVAR :: 
+  "NAME \<Rightarrow> bool \<Rightarrow> 'a itself \<Rightarrow> 'm itself \<Rightarrow> ('a, 'm :: VALUE) PVAR" where
+"MkPVAR n s a t = Abs_PVAR (n, s)"
+
+abbreviation pvname :: "('a, 'm :: VALUE) PVAR \<Rightarrow> NAME" where
+"pvname x \<equiv> fst (Rep_PVAR x)"
+
+abbreviation pvaux :: "('a, 'm :: VALUE) PVAR \<Rightarrow> bool" where
+"pvaux x \<equiv> snd (Rep_PVAR x)"
+
+lemma pvname_MkPVAR [simp]:
+  "pvname (MkPVAR n s a m) = n"
+  by (simp add:MkPVAR_def)
+
+lemma pvaux_MkPVAR [simp]:
+  "pvaux (MkPVAR n s a m) = s"
+  by (simp add:MkPVAR_def)
+
+definition pvundash :: "('a, 'm :: VALUE) PVAR \<Rightarrow> ('a, 'm :: VALUE) PVAR" where
+"pvundash v = Abs_PVAR (MkName (name_str (pvname v)) (dashes (pvname v) - 1) (subscript (pvname v)), pvaux v)"
+
+definition pvdash :: "('a, 'm :: VALUE) PVAR \<Rightarrow> ('a, 'm :: VALUE) PVAR" where
+"pvdash v = Abs_PVAR (MkName (name_str (pvname v)) (dashes (pvname v) + 1) (subscript (pvname v)), pvaux v)"
+
+text {* This function performs a type erasure on the variable. *}
+
+definition PVAR_VAR :: "('a, 'm) PVAR \<Rightarrow> ('m :: VALUE) VAR" ("[_]\<^sub>*") where
+"PVAR_VAR v = MkVar (pvname v) (TypeU TYPE('a)) (pvaux v)"
+
+definition VAR_PVAR :: "('m :: VALUE) VAR \<Rightarrow> ('a, 'm) PVAR" where
+"VAR_PVAR v = Abs_PVAR (name v, aux v)"
+
+lemma PVAR_VAR_inv [simp]: 
+  "VAR_PVAR [v]\<^sub>* = v"
+  by (simp add:PVAR_VAR_def VAR_PVAR_def)
+
+lemma VAR_PVAR_inv [simp]: 
+  "vtype x = TYPEU('a) \<Longrightarrow> [VAR_PVAR x :: ('a, 'm :: VALUE) PVAR]\<^sub>* = x"
+  apply (case_tac x)
+  apply (auto simp add:PVAR_VAR_def VAR_PVAR_def MkVar_def)
+done
+
+lemma PVAR_VAR_pvundash [simp]:
+  "[pvundash x]\<^sub>* = undash [x]\<^sub>*"
+  by (auto simp add:PVAR_VAR_def undash_def pvundash_def)
+
+lemma PVAR_VAR_pvdash [simp]:
+  "[pvdash x]\<^sub>* = dash [x]\<^sub>*"
+  by (auto simp add:PVAR_VAR_def dash_def pvdash_def)
+
+abbreviation "PUNDASHED     \<equiv> {x. PVAR_VAR x \<in> UNDASHED}"
+abbreviation "PDASHED       \<equiv> {x. PVAR_VAR x \<in> DASHED}"
+abbreviation "PDASHED_TWICE \<equiv> {x. PVAR_VAR x \<in> DASHED_TWICE}"
+
+subsection {* Adapting Renaming *}
+
+definition Rep_VAR_RENAME_poly :: 
+  "'m VAR_RENAME \<Rightarrow> ('a, 'm :: VALUE) PVAR \<Rightarrow> ('a, 'm) PVAR" where
+"Rep_VAR_RENAME_poly ss x \<equiv> VAR_PVAR (\<langle>ss\<rangle>\<^sub>s [x]\<^sub>*)"
+
+notation Rep_VAR_RENAME_poly ("\<langle>_\<rangle>\<^sub>s\<^sub>*")
+
+lemma PVAR_VAR_vtype [simp]:
+  "vtype [x :: ('a, 'm :: VALUE) PVAR]\<^sub>* = TYPEU('a)"
+  by (simp add:PVAR_VAR_def)
+
+lemma PVAR_VAR_RENAME [simp]: 
+  "[\<langle>ss\<rangle>\<^sub>s\<^sub>* x]\<^sub>* = \<langle>ss\<rangle>\<^sub>s [x]\<^sub>*"
+  by (simp add:Rep_VAR_RENAME_poly_def)
+
+end
+
